test-suite/cofix.v
@@ -1,0 +1,7 @@
+Require Import Template.Template.
+Require Import Streams.
+
+CoFixpoint ones := Cons 1 ones.
+
+Quote Recursively Definition q_ones := ones.
+
