test-suite/proj.v
@@ -1,0 +1,18 @@
+Require Import Template.Template.
+
+Set Primitive Projections.
+
+Record Eq (A : Type) := { eq : A -> A -> bool }.
+
+Goal forall {A} {e : Eq A} x y, e.(eq _) x y = eq _ e x y.
+Proof.
+  intros.
+  match goal with
+   |- ?T => quote_term T (fun x => pose (qgoal:=x))
+  end.
+Show.
+  match goal with
+    H:= context [Ast.tProj "Top.proj.eq" _] |- _ => idtac
+  end.
+  reflexivity.
+Qed.
