theories/TemplateCoqCompiler.v
@@ -1,3 +1,3 @@
-Require Import String Template.Ast BinNat.
+Require Import String Template.Ast.
 
 Declare ML Module "template_coq_plugin".
